% \begin{figure}
%     \begin{tikzpicture}[scale=5]
%         \draw
%         let
%             \p{P} = (0, 0),
%             \p{p} = (3, 0),
%             \p{Q} = (0, 1),
%             \p{q} = (3, 0),
%             \p{R} = (0, 1),
%             \p{r} = (3, 0),
%             \p{S} = (0, 0),
%             \p{s} = (3, 0),
%         in
%             node[inner sep=0] (P)  at (\p{P}) {$\bullet$}
%             node[inner sep=0] (p)  at ({\x{P}+\x{p}/3}, {\y{P}+\y{p}/3}) {}
%             node[inner sep=0] (Q)  at ({\x{Q}},       {\y{Q}}) {$\bullet$}
%             node[inner sep=0] (q)  at ({\x{Q}+\x{q}/3}, {\y{Q}+\y{q}/3}) {}
%             node[inner sep=0] (R)  at (\p{R}) {$\bullet$}
%             node[inner sep=0] (r)  at ({\x{R}+\x{r}/3}, {\y{R}+\y{r}/3}) {}
%             node[inner sep=0] (S)  at ({\x{S}},       {\y{S}}) {$\bullet$}
%             node[inner sep=0] (s)  at ({\x{S}+\x{s}/3}, {\y{S}+\y{s}/3}) {};
%         \draw[-latex] (P) node[below left] {$P = 0$} -- (p) node[midway, below] {$\vec p = 3$};
%         \draw[-latex] (Q) node[above right] {$Q = i$} -- (q) node[midway, above] {$\vec q = 3$};
%         \draw[-latex] (R) node[above left] {$R = i$} -- (r) node[midway, below] {$\vec r = 3$};
%         \draw[-latex] (S) node[below right] {$S = 0$} -- (s) node[midway, above] {$\vec s = 3$};
%         \draw[domain=0:1, samples=\samplesTikz, variable=\t]
%         let
%             \p{P} = (0, 0),
%             \p{p} = (3, 0),
%             \p{Q} = (0, 1),
%             \p{q} = (3, 0),
%             \p{R} = (0, 1),
%             \p{r} = (3, 0),
%             \p{S} = (0, 0),
%             \p{s} = (3, 0),
%         in
%         % let
%         %     \p{P} = (0, 0),
%         %     \p{p} = (3, 0),
%         %     \p{Q} = (3, 2),
%         %     \p{q} = (0, -2),
%         %     \p{R} = (0, 3),
%         %     \p{r} = (3, 0),
%         %     \p{S} = (2, -1),
%         %     \p{s} = (0, -2)
%         % in
%         plot (
%             {   \x{P} + \x{p}*(\t) + (3*\x{Q} - 3*\x{P} - 2*\x{p} - \x{q})*(\t)*(\t) + (2*\x{P} - 2*\x{Q} + \x{p} + \x{q})*(\t)*(\t)*(\t)   },
%             {   \y{P} + \y{p}*(\t) + (3*\y{Q} - 3*\y{P} - 2*\y{p} - \y{q})*(\t)*(\t) + (2*\y{P} - 2*\y{Q} + \y{p} + \y{q})*(\t)*(\t)*(\t)   }
%         )
%         plot (
%             {   \x{R} + \x{r}*(\t) + (3*\x{S} - 3*\x{R} - 2*\x{r} - \x{s})*(\t)*(\t) + (2*\x{R} - 2*\x{S} + \x{r} + \x{s})*(\t)*(\t)*(\t)   },
%             {   \y{R} + \y{r}*(\t) + (3*\y{S} - 3*\y{R} - 2*\y{r} - \y{s})*(\t)*(\t) + (2*\y{R} - 2*\y{S} + \y{r} + \y{s})*(\t)*(\t)*(\t)   }
%         );
%     \end{tikzpicture}
%     \caption{Splines $\Lspline_{0,i,3,3}$ and $\Lspline_{i,0,3,3}$}
%     \label{fig:spline2}
% \end{figure}
given:
$$\begin{aligned}
	\Lspline_1(t) = \Lspline_{PQpq}(t) =& P + pt + T_1t^2 + U_1t^3 & \hspace{1cm}
	\Lspline_2(u) = \Lspline_{RSrs}(u) =& R + ru + T_2u^2 + U_2u^3 \\
	T_1 :=& (3Q-3P-2p-q) & \hspace{1cm}
	T_2 :=& (3S-3R-2r-s) \\
	U_1 :=& (2P-2Q+p+q)  & \hspace{1cm}
	U_2 :=& (2R-2S+r+s) \\
\end{aligned}$$
% separate into coordinates:
$$\begin{aligned}
%     P_x + p_xt + T_{1x}t^2 + U_{1x}t^3 =& \Lspline_2(u)_x & \hspace{1cm}
%     R_x + r_xu + T_{2x}u^2 + U_{2x}u^3 =& \Lspline_1(t)_x \\
%     P_y + p_yt + T_{1y}t^2 + U_{1y}t^3 =& \Lspline_2(u)_y & \hspace{1cm}
%     R_y + r_yu + T_{2y}u^2 + U_{2y}u^3 =& \Lspline_1(t)_y \\
% \end{aligned}$$
% combine again:
% $$\begin{aligned}
%     \frac{U_{1y}}{U_{1x}}\left(P_x + p_xt + T_{1x}t^2 + U_{1x}t^3\right) =& \frac{U_{1y}}{U_{1x}}\Lspline_2(u)_x & \hspace{1cm}
%     \frac{U_{2y}}{U_{2x}}\left(R_x + r_xu + T_{2x}u^2 + U_{2x}u^3\right) =& \frac{U_{2y}}{U_{2x}}\Lspline_1(t)_x \\
	w_{1y} :=& \frac{U_{1y}}{U_{1x}} & \hspace{1cm}
	w_{2y} :=& \frac{U_{2y}}{U_{2x}} \\
% \end{aligned}$$
% restructure:
% $$\begin{aligned}
%     (w_{1y}P_x - P_y) + & & \hspace{1cm}
%     (w_{2y}R_x - R_y) + & \\
%     (w_{1y}p_x - p_y)t + & & \hspace{1cm}
%     (w_{2y}r_x - r_y)u + & \\
%     (w_{1y}T_{1x} - T_{1y})t^2 =& w_{1y}\Lspline_2(u)_x & \hspace{1cm}
%     (w_{2y}T_{2x} - T_{2y})u^2 =& w_{2y}\Lspline_1(t)_x \\
	V_{10} :=& \frac{ w_{1y}P_x - P_y }{ w_{1y}T_{1x} - T_{1y} } & \hspace{1cm}
	V_{20} :=& \frac{ w_{2y}R_x - R_y }{ w_{2y}T_{2x} - T_{2y} } \\
	V_{11} :=& \frac{ w_{1y}p_x - p_y }{ w_{1y}T_{1x} - T_{1y} } & \hspace{1cm}
	V_{21} :=& \frac{ w_{2y}r_x - r_y }{ w_{2y}T_{2x} - T_{2y} } \\
% \end{aligned}$$
% quadratic:
% $$\begin{aligned}
%     w_{1y}\Lspline_2(u)_x =& V_{10} + V_{11}t + t^2 & \hspace{1cm}
%     w_{2y}\Lspline_1(t)_x =& V_{20} + V_{21}u + u^2 \\
%     0 =& t^2 + tV_{11} + V_{10} - W_{12}\Lspline_2(u)_x & \hspace{1cm}
%     0 =& u^2 + uV_{21} + V_{20} - W_{22}\Lspline_1(t)_x \\
	W_{10} :=& -\frac{V_{11}}{2} & \hspace{1cm}
	W_{20} :=& -\frac{V_{21}}{2} \\
	W_{11} :=& \left(\frac{V_{11}}{2}\right)^2 - V_{10} & \hspace{1cm}
	W_{21} :=& \left(\frac{V_{21}}{2}\right)^2 - V_{20} \\
	W_{12} :=& \frac{w_{1y}}{ w_{1y}T_{1x}-T_{1y} } & \hspace{1cm}
	W_{22} :=& \frac{w_{2y}}{ w_{2y}T_{2x}-T_{2y} } \\
	t =& W_{10} \pm \sqrt{
		W_{11} + W_{12}\Lspline_2(u)_x
	} & \hspace{1cm}
	u =& W_{20} \pm \sqrt{
		W_{21} + W_{22}\Lspline_1(t)_x
	} \\
% \end{aligned}$$
%     %     combine and die:
%     %     $$\begin{aligned}
%     %         t = W_{10} \pm& \sqrt{
%     %             W_{11} + W_{12}\Lspline_2\left(
%     %             W_{20} \pm \sqrt{
%     %                 W_{21} + W_{22}\Lspline_1(t)_x
%     %             }
%     %             \right)_x
%     %         } \\
%     %         M(t) := &\sqrt{ W_{21} + W_{22}\Lspline_1(t)_x } \\
%     %         t = W_{10} \pm& \sqrt{
%     %             W_{11} + W_{12}\Lspline_2\left(
%     %                 W_{20} \pm M(t)
%     %             \right)_x
%     %         } \\
%     %         t = W_{10} \pm& \sqrt{
%     %             W_{11} +
%     %             W_{12}\left(
%     %             R +
%     %             r  \left( W_{20} \pm M(t) \right) + %...\right. }\\&\sqrt{ \left. ...
%     %             T_2\left( W_{20} \pm M(t) \right)^2 + %...\right. }\\&\sqrt{ \left. ...
%     %             U_2\left( W_{20} \pm M(t) \right)^3
%     %             \right)
%     %         } \\
%     %         (t - W_{10})^2 = &W_{11} + W_{12}\left(
%     %             R +
%     %             r  \left( W_{20} \pm M(t) \right) +
%     %             T_2\left( W_{20} \pm M(t) \right)^2 +
%     %             U_2\left( W_{20} \pm M(t) \right)^3
%     %         \right) \\
%     %         \frac{(t - W_{10})^2 - W_{11}}{W_{12}} = &
%     %             R + r  W_{20} \pm r M(t)
%     %             +    T_2W_{20}^2
%     %             \pm 2T_2W_{20}M(t)
%     %             +    T_2      M^2(t)
%     %         \\ &
%     %             +    U_2W_{20}^3
%     %             \pm 3U_2W_{20}^2M(t)
%     %             +   3U_2W_{20}  M^2(t)
%     %             \pm  U_2        M^3(t)
%     %         \\
%     %         \frac{t^2}{W_{12}} - 2t\frac{W_{10}}{W_{12}} + \frac{W_{10}^2 - W_{11}}{W_{12}} = &
%     %             R
%     %             +    r  W_{20}
%     %             +    T_2W_{20}^2
%     %             +    U_2W_{20}^3
%     %         \\ &
%     %             \pm  r          M(t)
%     %             \pm 2T_2W_{20}  M(t)
%     %             \pm 3U_2W_{20}^2M(t)
%     %             +    T_2        M^2(t)
%     %             +   3U_2W_{20}  M^2(t)
%     %             \pm  U_2        M^3(t)
%     %         \\
%     %         W_3 :=& \frac{W_{10}^2 - W_{11}}{W_{12}} - R - rW_{20} - T_2W_{20}^2 - U_2W_{20}^3 \\
%     %         \frac{(t - W_{10})^2 - W_{11}}{W_{12}} + W_3 =
%     %         & M(t)\left(
%     %             \pm  r
%     %             \pm 2T_2W_{20}
%     %             \pm 3U_2W_{20}^2
%     %         + M(t)\left(
%     %                  T_2
%     %             +   3U_2W_{20}
%     %             \pm  U_2M(t)
%     %         \right)
%     %         \right) \\
%     %         W_4 := & \pm r \pm 2T_2W_{20} \pm 3U_2W_{20}^2 \\
%     %         W_5 := & T_2 + 3U_2W_{20} \\
%     %         \frac{(t - W_{10})^2 - W_{11}}{W_{12}} + W_3 =
%     %         & M(t)\left( W_4
%     %         + M(t)\left(
%     %             W_5 \pm U_2M(t)
%     %         \right)
%     %         \right) \\
%     %         \left( \frac{(t - W_{10})^2 - W_{11}}{W_{12}} + W_3 \right)^2 =
%     %         & M^2(t)( W_4
%     %             + M(t)(
%     %                 W_5 \pm U_2M(t)
%     %             )
%     %         )^2 \\
%     %         \frac{((t - W_{10})^2 - W_{11})^2}{W_{12}^2} \\
%     %         - 2\frac{(t - W_{10})^2 - W_{11}}{W_{12}}W_3 + W_3^2 =
%     %         & M^2(t)( W_4^2 + 2W_4M(t)(
%     %             W_5 \pm U_2M(t)
%     %             ) + M^2(t)(
%     %                 W_5^2 \pm 2W_5U_2M(t) + U_2^2M^2(t)
%     %             )
%     %         ) \\
%     %         \frac{(t - W_{10})^4}{W_{12}^2} - \frac{2(t - W_{10})^2W_{11}}{W_{12}^2} + \frac{W_{11}^2}{W_{12}^2} \\
%     %         - \frac{2(t - W_{10})^2W_3}{W_{12}} + \frac{2W_{11}W_3}{W_{12}} + W_3^2 =
%     %         &   M^2(t)W_4^2 + 2M^2(t)W_4M(t)W_5 \pm 2M^2(t)W_4M(t)U_2M(t) + \\
%     %         &   M^2(t)M^2(t)W_5^2 \pm 2M^2(t)M^2(t)W_5U_2M(t) + M^2(t)M^2(t)U_2^2M^2(t) \\
%     %         \frac{(t - W_{10})^4}{W_{12}^2} - \frac{2(t - W_{10})^2W_{11}}{W_{12}^2} + \frac{W_{11}^2}{W_{12}^2} \\
%     %         - \frac{2(t - W_{10})^2W_3}{W_{12}} + \frac{2W_{11}W_3}{W_{12}} + W_3^2 =
%     %         &   M^2(t)W_4^2 + 2M^3(t)W_4W_5 \pm 2M^4(t)W_4U_2 + M^4(t)W_5^2 \pm 2M^5(t)W_5U_2 + M^6(t)U_2^2 \\
%     %     \end{aligned}$$
% different approach:
% $$\begin{aligned}
%     \Lspline_1(t) =& \Lspline_{PQpq}(t) = P + pt + (3Q-3P-2p-q)t^2 + (2P-2Q+p+q)t^3 \\
%     \Lspline_2(u) =& \Lspline_{RSrs}(u) = R + ru + (3S-3R-2r-s)u^2 + (2R-2S+r+s)u^3 \\
%     \nLspline(t, u) =& \left|\Lspline_{PQpq}(t) - \Lspline_{RSrs}(u)\right| \\
%     0 = &(\Lspline_1(t)_x - \Lspline_2(u)_x)^2 + (\Lspline_1(t)_y - \Lspline_2(u)_y)^2 \\
%     0 = &\left(P_x + p_xt + T_{1x}t^2 + U_{1x}t^3 - R_x - r_xu - T_{2x}u^2 - U_{2x}u^3\right)^2  \\
%       + &\left(P_y + p_yt + T_{1y}t^2 + U_{1y}t^3 - R_y - r_yu - T_{2y}u^2 - U_{2y}u^3\right)^2 \\
\end{aligned}$$
then I just gave in and implemented an approximating algorithm that used gradient descent with mean slope.
